%% LyX 2.3.0 created this file.  For more info, see http://www.lyx.org/.
%% Do not edit unless you really know what you are doing.
\documentclass[english]{article}
\usepackage[T1]{fontenc}
\usepackage[latin9]{inputenc}
\usepackage{mathtools}
\usepackage{amsmath}
\usepackage{amssymb}
\usepackage{cancel}

\makeatletter

%%%%%%%%%%%%%%%%%%%%%%%%%%%%%% LyX specific LaTeX commands.
%% Because html converters don't know tabularnewline
\providecommand{\tabularnewline}{\\}

\makeatother

\usepackage{babel}
\begin{document}

\title{A Dynamic Dependent Type Theory with Type-in-Type and Recursion}
\maketitle

\section{Type Soundness or Blame}

The proof follows the standard structure:
\begin{itemize}
\item All judgments respect weakening and well typed substitution
\item Most judgments are marked with types to make subject reduction obvious
(assuming the substitution lemma)
\item definitional equality is defined in terms par-reductions, which (via
confluence)
\begin{itemize}
\item gives transitivity to equality
\item means that type constructors are unique, $\ast\bcancel{\equiv}\Pi$
\end{itemize}
\item for preservation, function elimination is the only interesting case 
\begin{itemize}
\item the stack of casts is inspected, all casts are values (usually either
$\star$ or $\Pi$ )
\begin{itemize}
\item if all casts are $\Pi$ then coersions can be calculated and a reduction
can step
\item if any casts are not $\Pi$ there is a specific source location and
observation to blame 
\end{itemize}
\end{itemize}
\end{itemize}

\subsection{Structural Properties}

\subsubsection{Weakening}

For any derivation of $H\vdash A:\star$ the following rules are admissible:

\[
\frac{H,H'\vdash}{H,x:A,H'\vdash}
\]

\[
\frac{H,H'\vdash b:B}{H,x:A,H'\vdash b:B}
\]

\[
\frac{H,H'\vdash e:\overline{\star}}{H,x:A,H'\vdash e:\overline{\star}}
\]

\[
\frac{H,H'\vdash b\equiv b':B}{H,x:A,H'\vdash b\equiv b':B}
\]

\[
\frac{H,H'\vdash b\Rrightarrow_{*}b':B}{H,x:A,H'\vdash b\Rrightarrow_{*}b':B}
\]

\[
\frac{H,H'\vdash b\Rrightarrow b':B}{H,x:A,H'\vdash b\Rrightarrow b':B}
\]

\[
\frac{H,H'\vdash e\Rrightarrow e':\overline{\star}}{H,x:A,H'\vdash e\Rrightarrow e':\overline{\star}}
\]

\[
\frac{H,H'\vdash o\Rrightarrow o'}{H,x:A,H'\vdash o\Rrightarrow o'}
\]


\subsection{Substitution}

\subsubsection{$\Rrightarrow$ is reflexive}

The following rules are admissible:

\[
\frac{H\vdash a:A}{H\vdash a\Rrightarrow\,a:A}
\]

\[
\frac{H\vdash e:\overline{\star}}{H\vdash e\Rrightarrow e':\overline{\star}}
\]

\[
\frac{H\vdash}{H\vdash o\Rrightarrow o}
\]

by mutual induction

\subsubsection{Context substitution}

For any derivation of $H\vdash a:A$ the following rules are admissible:

\[
\frac{H,x:A,H'\vdash}{H,H'\left[x\coloneqq A\right]\vdash}
\]

\[
\frac{H,x:A,H'\vdash b:B}{H,H'\left[x\coloneqq a\right]\vdash b\left[x\coloneqq a\right]\,:\,B\left[x\coloneqq a\right]}
\]

\[
\frac{H,x:A,H'\vdash e:\overline{\star}}{H,H'\left[x\coloneqq a\right]\vdash e\left[x\coloneqq a\right]\,:\overline{\star}}
\]

\[
\frac{H,x:A,H'\vdash e:\overline{\star}}{H,H'\left[x\coloneqq a\right]\vdash e\left[x\coloneqq a\right]\,:\overline{\star}}
\]

\[
\frac{H,x:A,H'\vdash b\equiv b':B}{H,H'\left[x\coloneqq a\right]\vdash b\left[x\coloneqq a\right]\equiv b'\left[x\coloneqq a\right]:B\left[x\coloneqq a\right]}
\]

\[
\frac{H,x:A,H'\vdash b\Rrightarrow_{*}b':B}{H,H'\left[x\coloneqq a\right]\vdash b\left[x\coloneqq a\right]\Rrightarrow_{*}b'\left[x\coloneqq a\right]:B\left[x\coloneqq a\right]}
\]

\[
\frac{H,x:A,H'\vdash b\Rrightarrow b':B}{H,H'\left[x\coloneqq a\right]\vdash b\left[x\coloneqq a\right]\Rrightarrow b'\left[x\coloneqq a\right]:B\left[x\coloneqq a\right]}
\]

\[
\frac{H,x:A,H'\vdash e\Rrightarrow e':\overline{\star}}{H,H'\left[x\coloneqq a\right]\vdash e\left[x\coloneqq a\right]\Rrightarrow e'\left[x\coloneqq a\right]\,:\overline{\star}}
\]

\[
\frac{H,x:A,H'\vdash o\Rrightarrow o'}{H,H'\left[x\coloneqq a\right]\vdash o\left[x\coloneqq a\right]\Rrightarrow o'\left[x\coloneqq a\right]}
\]

\[
\frac{H,x:A,H'\vdash b\sim b':B}{H,H'\left[x\coloneqq a\right]\vdash b\left[x\coloneqq a\right]\sim b'\left[x\coloneqq a\right]:B\left[x\coloneqq a\right]}
\]

\[
\frac{H,x:A,H'\vdash e\sim e':\overline{\star}}{H,H'\left[x\coloneqq a\right]\vdash e\left[x\coloneqq a\right]\sim e'\left[x\coloneqq a\right]:\overline{\star}}
\]

\[
\frac{H,x:A,H'\vdash e\,Elim_{\Pi}y:e_{A}.e_{B}}{H,H'\left[x\coloneqq a\right]\vdash e\left[x\coloneqq a\right]\,Elim_{\Pi}y:e_{A}\left[x\coloneqq a\right].e_{B}\left[x\coloneqq a\right]}
\]

\[
\frac{H,x:A,H'\vdash e\,Elim_{\star}}{H,H'\left[x\coloneqq a\right]\vdash e\left[x\coloneqq a\right]\,Elim_{\star}}
\]

by mutual induction on the derivations with reflexivity lemmas. 

\subsection{Computation}

\subsubsection{$\Rrightarrow$ $Elim_{\star}$}

if $e\,Elim_{\star}$ and $e\Rrightarrow e'$ then $e'\,Elim_{\star}$

by induction on $Elim_{\star}$

\subsubsection{$\Rrightarrow$-substitution }

For any $a\Rrightarrow a'$. The following rules are admissible:

\[
\frac{b\Rrightarrow b'}{b\left[x\coloneqq a\right]\Rrightarrow b'\left[x\coloneqq a'\right]}
\]

\[
\frac{e\Rrightarrow e}{e\left[x\coloneqq a\right]\Rrightarrow e'\left[x\coloneqq a'\right]}
\]

\[
\frac{e\Rrightarrow e'\quad e\left[x\coloneqq a\right]\,Elim_{\Pi}x:e_{A}\left[x\coloneqq a\right].e_{B}\left[x\coloneqq a\right]}{e_{A}\Rrightarrow e_{A}'\quad e_{B}\Rrightarrow e_{B}'\quad e'\left[x\coloneqq a'\right]\,Elim_{\Pi}x:e_{A}'\left[x\coloneqq a'\right].e_{B}'\left[x\coloneqq a'\right]}
\]

by mutual induction on the derivations

\subsubsection{$\Rrightarrow$ preserves type in destination}

\[
\frac{H\vdash a\Rrightarrow a':A}{H\vdash a':A}
\]

Since the apparent type of $a$ will at most $A\Rrightarrow A'$ (by
$\Rrightarrow$-substitution) so $H\vdash A\equiv A':\star$ , and
follows from conversion

\subsubsection{$\Rrightarrow_{\ast}$ preserves type}

The following rule is admissible:

\[
\frac{H\vdash a\Rrightarrow_{\ast}\,a':A}{H\vdash a:A}
\]

by induction

\[
\frac{H\vdash a\Rrightarrow_{\ast}\,a':A}{H\vdash a':A}
\]

by induction

\subsubsection{$\sim$ preserves type}

The following rules are admissible:

\[
\frac{H\vdash a\sim a':A}{H\vdash a':A}
\]

by induction

\subsubsection{$\equiv$ preserves type}

The following rules are admissible:

\[
\frac{H\vdash a\equiv\,a':A}{H\vdash a:A}
\]

\[
\frac{H\vdash a\equiv\,a':A}{H\vdash a':A}
\]

by the def of $\Rrightarrow_{\ast}$ 

\subsubsection{def of $-^{*}$ }

there is a maximal par-reduction step that can be computed for every
syntactic form defined:

\begin{tabular}{rll}
$\star^{*}$ & $=\star$ & $a^{*}\rightarrow a$\tabularnewline
$\left(\Pi x:A.B\right)^{*}$ & $=\Pi x:A^{*}.B^{*}$ & \tabularnewline
$\left(a_{h}::e\right)^{*}$ & $=a_{h}^{*}::e^{*}$ & \tabularnewline
$\left(\left(\mathsf{fun}\,f.\,y.b\right)::e\,a\right)^{*}$ & $=\left(b^{*}\left[f\coloneqq\left(\mathsf{fun}\,f.\,x.b^{*}\right),x\coloneqq a^{*}::e_{A}^{*}\right]::e_{B}^{*}\left[x\coloneqq a^{*}\right]\right)$
if $e\,Elim_{\Pi}x:e_{A}.e_{B}$ & $a_{h}^{*}\rightarrow a$\tabularnewline
$\left(b\,a\right)^{*}$ & $=b^{*}\,a^{*}$ otherwise & \tabularnewline
$x^{*}$ & $=x$ & \tabularnewline
$\left(\mathsf{fun}\,f.\,x.b\right)^{*}$ & $=\mathsf{fun}\,f.\,x.b^{*}$ & \tabularnewline
$\left(e=_{l,o}A\right)^{*}$ & $=e^{*}=_{l,o^{*}}A^{*}$ & $e^{*}\rightarrow e$\tabularnewline
$.^{*}$ & $=.$ & $o^{*}\rightarrow o$\tabularnewline
$\left(o.arg\right)^{*}$ & $=o^{*}.arg$ & \tabularnewline
$\left(o.bod[b]\right)^{*}$ & $=o^{*}.bod[b^{*}]$ & \tabularnewline
\end{tabular}

\subsubsection{$-^{*}$ $Elim_{\star}$}

if $e\,Elim_{\star}$ then $e^{*}\,Elim_{\star}$ 

by induction on $Elim_{\star}$

\subsubsection{$-^{*}$ $Elim_{\Pi}$}

if $e\,Elim_{\Pi}x:e_{A}.e_{B}$ then $e^{*}\,Elim_{\Pi}x:e_{A}^{*}.e_{B}^{*}$ 

by induction on $Elim_{\Pi}$


\subsubsection{$-^{*}$ is maximal}
\begin{itemize}
\item if $a\Rrightarrow a'$ then $a'\Rrightarrow a^{*}$ 
\item if $e\Rrightarrow e'$ then $e'\Rrightarrow e^{*}$ 
\item if $o\Rrightarrow o'$ then $o'\Rrightarrow o^{*}$ 
\end{itemize}
by mutual induction on $\Rrightarrow$ relations, interesting cases
include
\begin{itemize}
\item $\Pi C\Rrightarrow$ since if $e\,Elim_{\Pi}x:e_{A}.e_{B}$ then $e^{*}\,Elim_{\Pi}x:e_{A}^{*}.e_{B}^{*}$ 
\item $\Pi E\Rrightarrow$ , $b\,a\Rrightarrow b'\,a'$
\begin{itemize}
\item if the elimination is not possible with $b$, follows from induction
\item if the elimination is possible with $b$, it will still be possible
with $b'$ since, by induction $b\Rrightarrow b'$ 
\end{itemize}
\end{itemize}

\subsubsection{$\Rrightarrow$ is confluent}

if $H\vdash a\Rrightarrow b:A$ and $H\vdash a\Rrightarrow b':A$
then there exists $c$ such that 

$H\vdash b\Rrightarrow c:A$ and $\Gamma\vdash b'\Rrightarrow c:A$

by the maximality of $-^{*}$

\subsubsection{$\Rrightarrow_{\ast}$ is transitive}

The following rule is admissible:

\[
\frac{H\vdash a\Rrightarrow_{\ast}\,b:A\quad H\vdash b\Rrightarrow_{\ast}c:A}{H\vdash a\Rrightarrow_{\ast}\,c:A}\,\textrm{\ensuremath{\Rrightarrow\ast}-trans}
\]

by induction

\subsubsection{$\Rrightarrow_{\ast}$ is confluent}

if $H\vdash a\Rrightarrow_{\ast}\,b:A$ and $H\vdash a\Rrightarrow_{\ast}\,b':A$
then there exists $c$ such that 

$H\vdash b\Rrightarrow_{\ast}\,c:A$ and $H\vdash b'\Rrightarrow_{\ast}\,c:A$

Follows from $\textrm{\ensuremath{\Rrightarrow\ast}-trans}$ and the
confluence of $\Rrightarrow$ using standard techniques

\subsubsection{$\sim$Equivalence}

The following rules are admissible:

\[
\frac{\,}{a\sim a'}
\]

\[
\frac{a\sim a'}{a'\sim a}
\]

\[
\frac{a\sim a'\quad a'\sim a''}{a'\sim a''}
\]

each by induction

\subsubsection{$\sim$ commutes with \textmd{$\Rrightarrow$, $\Rrightarrow_{\ast}$}}

The following rules are admissible:

\[
\frac{a\Rrightarrow a'\quad a\sim b}{b\Rrightarrow b'\quad a'\sim b'}
\]

\[
\frac{H\vdash a\Rrightarrow_{\ast}a':A\quad a\sim b}{H\vdash b\Rrightarrow_{\ast}b':A\quad a'\sim b'}
\]

both by induction (observations can be ignored since $\Rrightarrow$
is reflexive)

\subsubsection{$\equiv$Equivalence}

The following rule is admissible:

\[
\frac{H\vdash a:A}{H\vdash a\equiv a:A}\,\textrm{\ensuremath{\equiv}-refl}
\]

by $\,\textrm{\ensuremath{\Rrightarrow\ast}-refl}$and $\textrm{\ensuremath{\sim}-refl}$

The following rule is admissible:

\[
\frac{H\vdash a\equiv a':A}{H\vdash a'\equiv a:A}\,\textrm{\ensuremath{\equiv}-sym}
\]

by $\sim$Equivalence

The following rule is admissible:

\[
\frac{H\vdash a\equiv b:A\qquad H\vdash b\equiv c:A}{H\vdash a\equiv c:A}\,\textrm{\ensuremath{\equiv}-trans}
\]

by the confluence of $\Rrightarrow_{\ast}$and $\sim$ commutativity

\subsubsection{$\rightsquigarrow$ preserves type}

For any derivations of $H\vdash a:A$, $a\rightsquigarrow a'$,

\[
H\vdash a':A
\]

since $\rightsquigarrow$ implies $\Rrightarrow$ and $\Rrightarrow$
preserves types

\subsection{Type constructors}

\subsubsection{Type constructors are stable over $\Rrightarrow$}
\begin{itemize}
\item if $\ast\Rrightarrow A$ then $A$ is $\ast$
\item if $\ast::e\Rrightarrow A_{h}::e'$ then $A_{h}$ is $\ast$
\item if $\Pi x:A.B\Rrightarrow C$ then $C$ is $\Pi x:A'.B'$ for some
$A',B'$
\item if $\Pi x:A.B::e\Rrightarrow C_{h}::e'$ then $C_{h}$ is $\Pi x:A'.B'$
for some $A',B'$
\end{itemize}
by induction on $\Rrightarrow$

\subsubsection{Type constructors are stable over $\Rrightarrow_{\ast}$}
\begin{itemize}
\item if $H\vdash\ast\Rrightarrow_{\ast}A:B$ then $A_{h}$ is $\ast$
\item if $H\vdash\ast::e\Rrightarrow_{\ast}A_{h}::e':B$ then $A_{h}$ is
$\ast$
\item if $H\vdash\Pi x:A.B\Rrightarrow_{\ast}C:D$ then $C$ is $\Pi x:A'.B'$
for some $A',B'$
\item if $H\vdash\Pi x:A.B::e\Rrightarrow_{\ast}C_{h}::e':D$ then $C_{h}$
is $\Pi x:A'.B'$ for some $A',B'$
\end{itemize}
by induction on $\Rrightarrow_{\ast}$ 

\subsubsection{Type constructors are stable over $\sim$}
\begin{itemize}
\item if $\ast\sim A$ then $A$ is $\ast$
\item if $\ast::e\sim A_{h}::e'$ then $A_{h}$ is $\ast$
\item if $\Pi x:A.B\sim C$ then $C$ is $\Pi x:A'.B'$ for some $A',B'$
\item if $\Pi x:A.B::e\sim C_{h}::e'$ then $C_{h}$ is $\Pi x:A'.B'$ for
some $A',B'$
\end{itemize}
by induction on $\sim$

\subsubsection{Type constructors definitionaly unique}

for any $H,A,B,C,e,e'$
\begin{itemize}
\item $H\vdash\ast\bcancel{\equiv}\Pi x:A.B\,:C$ 
\item $H\vdash\ast::e\bcancel{\equiv}\Pi x:A.B\,:C$ 
\item $H\vdash\ast\bcancel{\equiv}\Pi x:A.B::e\,:C$ 
\item $H\vdash\ast::e\bcancel{\equiv}\Pi x:A.B::e'\,:C$ 
\end{itemize}
from constructor stability

\subsection{Canonical forms}

If $\lozenge\vdash v_{h}\,:\Pi x:A.B$, then $v_{h}$ is $\mathsf{fun}\,f.\,x.b$,
since it is the only applicable rule

\subsection{Type simplification}

To minimize bookkeeping, when $\lozenge\vdash v_{eq}:\overline{\star}$
\begin{itemize}
\item $\star::v_{eq}$ can be said to simplify to $\star$ if each $v_{eq}$
simplifies to $\star$ (if it does not simplify there is a source
of blame)
\item $\Pi x:A.B::v_{eq}$ can be said to simplify to $\Pi x:A.B$ if each
$v_{eq}$ simplifies to $\star$ (if it does not simplify there is
a source of blame)
\end{itemize}

\subsection{Progress}

$\lozenge\vdash c:A$ implies that $c$ is a value, there exists $c'$
such that $c\rightsquigarrow c'$, or a static location can be blamed.
and $\lozenge\vdash e:\overline{\star}$ implies that $e$ is a value,
there exists $e'$ such that $e\rightsquigarrow e'$, or a static
location can be blamed

By mutual induction on the typing derivations with the help of the
canonical forms lemma

Explicitly:

cast typing
\begin{itemize}
\item $eq-ty-1$ by \textbf{induction}
\item $eq-ty-2$ by \textbf{induction}
\end{itemize}
term typing
\begin{itemize}
\item $c$ is typed by type-in-type. $c$ is $\star$, a value
\item $c$ is typed by $\Pi-ty$. $a$ is a value
\item $c$ is typed by the conversion rule, then by \textbf{induction}
\item $c$ is typed by the $apparent$ rule, then $c$ is $a_{h}::e$ by
each head typing. By induction $e$ is a value, there exists $e'$
such that $e\rightsquigarrow e'$. If there is blame that blame can
be used, if $e\rightsquigarrow e'$ preform the step. otherwise $e$
is a value:
\begin{itemize}
\item $a_{h}$ cannot be typed by the variable rule in the empty context
\item $a_{h}$ is typed by type-in-type. $a$ is $\star$.
\item $a_{h}$ is typed by $\Pi-ty$. $a$ is a value
\item $a_{h}$ is typed by $\Pi-\mathsf{fun}-ty$. $a$ is a value
\item $a_{h}$ is typed by $\Pi-app-ty$. Then $a_{h}$ is $b\,a$, and
there are derivations of $\lozenge\vdash b:\Pi x:A.B$, and $\lozenge\vdash a:A$
for some $A$ and $B$. By \textbf{induction} $a$ is a value, there
exists $a'$ such that $a\rightsquigarrow a'$, or blame and $b$
is a value or there exists $b'$ such that $b\rightsquigarrow b'$
or blame.
\begin{itemize}
\item if $b$ and $a$ are values, then $b$ is $b_{h}::v_{eq}$, where
$v_{eq}\uparrow$ is $\Pi x:A_{\uparrow}.B_{\uparrow}$ (or $v_{eq}\uparrow$
is $\Pi x:A_{\uparrow}.B_{\uparrow}::e$ , and by simplification $\Pi x:A_{\uparrow}.B_{\uparrow}$
or blame can be produced) (by \textbf{stability}) 
\begin{itemize}
\item if $v_{eq}\,Elim_{\Pi}\,x:e_{A}.e_{B}$ then $v_{eq}\downarrow$ is
$\Pi x:A_{\downarrow}.B_{\downarrow}$ (or $\Pi x:A_{\downarrow}.B_{\downarrow}::e$,
and by simplification $\Pi x:A_{\downarrow}.B_{\downarrow}$ or blame
can be produced) by \textbf{Canonical forms} $b_{h}$ is $\left(\mathsf{fun}\,f.\,x.b'\right)$
and the step is $\left(\left(\mathsf{fun}\,f.\,x.b\right)::v_{eq}\,v\right)::v_{eq}'\rightsquigarrow\left(b\left[f\coloneqq\left(\mathsf{fun}\,f.\,x.b\right),x\coloneqq v::e_{A}\right]::e_{B}'\left[x\coloneqq v\right]\right)$
(implicitly uses that $Elim_{\Pi}$is deterministic in its first argument)
\item if $v_{eq}\,\bcancel{Elim_{\Pi}}$ then there must exist $\left[\bcancel{\Pi}=_{l,o}\Pi x:A''.B''\right]\in v_{eq}$
(with simplification) and $l,o$ can be blamed 
\end{itemize}
\item if $b$ or $a$ can construct blame then $b\,a$ can use that blame
\item if $b$ is a value and $a\rightsquigarrow a'$ then $b\,a\rightsquigarrow b\,a'$
\item if $b\rightsquigarrow b'$ then $b\,a\rightsquigarrow b'\,a$
\end{itemize}
\end{itemize}
\end{itemize}

\subsection{Type Soundness}

For any well typed term in an empty context, no sequence of small
step reductions will cause a computation to ``get stuck'' without
blame. Either a final value will be reached, further reductions can
be taken, or blame is omitted. This follows by iterating the progress
and preservation lemmas.

\section{Elaboration Embeds Typing}

$\vdash m:M$, and $\vdash m\,Elab\,a$ then $\vdash M\,Elab\,A$,
$\vdash a:A$

Sketch (need to extend the hypothesis further to handle conversion):
\begin{itemize}
\item strengthen the hypothesis to $\varGamma\,Elab\,H$, $\varGamma\vdash m:M$,
and $H\vdash m\,Elab\,a$ then $H\vdash a:A$, $H\vdash M\,Elab\,A$
\item by induction if $\varGamma\,Elab\,H$, for all $x:M\in\varGamma$,
implies $x:A\in H$, $H\vdash M\,Elab\,A$
\item follows by induction on the typing derivation (of the base language)
\end{itemize}

\section{Elaboration Embeds Typing 2}

a better proposition would be 

$\vdash m:M$, then $\vdash m\,Elab\,a$ $\vdash M\,Elab\,A$, $\vdash a:A$

but this is technically incorrect since $\vdash(\lambda x.x)7:\mathbb{N}$,
but the Elaboration process is bidirectional.

\section{Computation resulting in blame cannot be typed in the surface language}

$\vdash a:A$ and $a$ blame then there is no $\vdash m:M$ such that
$\vdash M\,Elab_{\star,l}\,A$, and $\vdash m\,Elab_{A,l'}\,a$ 

Sketch: if $\vdash m:M$ then $\vdash a:A$ are elaborated without
source labels ($l,l'$ are superfluous) therefore blame is impossible
to construct

\section{Computation in the cast language respects computation in the surface
language}

$\vdash A:*$ and $\vdash M\,Elab_{\star,l}\,A$ then
\begin{enumerate}
\item if $A\rightsquigarrow_{*}*$ then $M\rightsquigarrow_{*}*$
\item if $A\rightsquigarrow_{*}\Pi x:B.C$ then $M\rightsquigarrow_{*}\Pi x:N.P$ 
\end{enumerate}
Sketch: evaluation is designed to be ``correct by construction''
. Casts and cast evaluation steps can be completely removed, resulting
in exactly the small steps of the surface language
\end{document}
