%% LyX 2.3.0 created this file.  For more info, see http://www.lyx.org/.
%% Do not edit unless you really know what you are doing.
\documentclass[english]{article}
\usepackage[T1]{fontenc}
\usepackage[latin9]{inputenc}
\usepackage{mathtools}
\usepackage{amsmath}
\usepackage{amssymb}
\usepackage{babel}
\begin{document}

\title{Type Soundness in an Intensional Dependent Type Theory with Type-in-Type,
Recursion and Data}

\maketitle
\textbf{There is an error in the parallel reduction that has not yet
been corrected}

\section{Examples}

logical unsoundness:

$\mathsf{fun}\,f:\left(x.x\right).\,x:\star.f\,x\qquad:\varPi x:\star.x$

\subsection*{some constructs}

while logically unsound, the language is extremely expressive. Conventional
data is representable:

$\mathsf{data}\,Unit.\,\mathsf{where}\,\left\{ tt.\rightarrow Unit\right\} $

~

$\mathsf{data}\,\mathbb{B}.\,\mathsf{where}\,\left\{ true.\rightarrow\mathbb{B}\,|\,false.\rightarrow\mathbb{B}\right\} $

~

$\mathsf{data}\,\mathbb{N}.\,\mathsf{where}\,\left\{ z.\rightarrow\mathbb{N}\,|\,suc\,x:\mathbb{N}.\rightarrow\mathbb{N}\right\} $

data abstraction allows some self-reference

$0\coloneqq z$

$1\coloneqq suc\,z$

~

$\mathsf{data}\,Vec\,A:\star,n:\mathbb{N}.\,\mathsf{where}\left\{ \begin{array}{cc}
nil\,A:\star. & \rightarrow Vec\,A\,0\\
cons\,A:\star,n:\mathbb{N},-:A,-:Vec\,A\,n. & \rightarrow Vec\,A\,\left(suc\,n\right)
\end{array}\right\} $

$rep_{\mathbb{B}}\coloneqq\mathsf{fun}\,f:\left(n.Vec\,\mathbb{B}\,n\right).\,n:\mathbb{N}.\mathsf{Case}_{n':\mathbb{N}\rightarrow Vec\,\mathbb{B}\,n'}\,n\,\mathsf{of}\left\{ z\Rightarrow nil\,\mathbb{B}\,|\,suc\,x\Rightarrow cons\,\mathbb{B}\,x\,true\,\left(f\,x\right)\right\} \qquad:\varPi n:\mathbb{N}.Vec\,\mathbb{B}\,n$

~

$\mathsf{data}\,Id\,A:\star,a_{1}:A,a_{2}:A.\,\mathsf{where}\,\left\{ refl\,A:\star,a:A.\rightarrow Id\,A\,a\,a\right\} $

$a_{1}=_{A}a_{2}\coloneqq Id\,A,a_{1},a_{2}$

~

$subst\coloneqq\lambda A.\lambda a_{1}.\lambda a_{2}.\lambda pr.\mathsf{Case}_{-:Id\,A,a_{1},a_{2}.\rightarrow\varPi C:\left(A\rightarrow\star\right).C\,a_{1}\rightarrow C\,a_{2}}\,pr\,\mathsf{of}\left\{ refl\,A:\star,a:A\Rightarrow\lambda C.\lambda x:C\,a.\,x\right\} $

$subst:\varPi A:\star.\varPi a_{1}:A.\varPi a_{2}:A.a_{1}=_{A}a_{2}\rightarrow\varPi C:\left(A\rightarrow\star\right).C\,a_{1}\rightarrow C\,a_{2}$

~

$\mathsf{data}\,\perp\,.\,\mathsf{where}\,\left\{ \,\right\} $

~

$\lnot A\coloneqq\varPi A:\star..A\rightarrow\perp$

~

$\lnot1=_{\mathbb{N}}0$ is provable (in a non trivial way):

$dec\coloneqq\lambda n.\mathsf{Case}_{-:\mathbb{N}.\rightarrow\star}\,pr\,\mathsf{of}\mathsf{of}\left\{ z\Rightarrow\perp\,|\,suc\,-\Rightarrow Unit\right\} \qquad:\mathbb{N}\rightarrow\star$

$\lambda pr.subst\,\mathbb{N}\,1\,0\,pr\,dec\,tt\qquad:\lnot1=_{\mathbb{N}}0$

Several larger examples are workable in prototype implementation

\section{Properties}

\subsection{Contexts}

\subsubsection{Sub-Contexts are well formed}

The following rules are admissible:

\[
\frac{\Gamma,\Gamma'\vdash}{\Gamma\vdash}
\]

\[
\frac{\Gamma,\Gamma'\vdash M:\sigma}{\Gamma\vdash}
\]

\[
\frac{\Gamma,\Gamma'\vdash M\Rrightarrow M':\sigma}{\Gamma\vdash}
\]

\[
\frac{\Gamma,\Gamma'\vdash M\Rrightarrow_{\ast}M':\sigma}{\Gamma\vdash}
\]

\[
\frac{\Gamma,\Gamma'\vdash M\equiv M':\sigma}{\Gamma\vdash}
\]

\[
\frac{\Gamma,\Gamma'\vdash\Delta:\overline{*}}{\Gamma\vdash}
\]

\[
\frac{\Gamma,\Gamma'\vdash\overline{M}:\Delta}{\Gamma\vdash}
\]

\[
\frac{\Gamma,\Gamma'\vdash\overline{M}\Rrightarrow\overline{M'}:\Delta}{\Gamma\vdash}
\]

by mutual induction on the derivations.

\subsubsection{Context weakening}

For any derivation of $\Gamma\vdash\sigma:\star$, the following rules
are admissible:

\[
\frac{\Gamma,\Gamma'\vdash}{\Gamma,x:\sigma,\Gamma'\vdash}
\]

\[
\frac{\Gamma,\Gamma'\vdash M:\tau}{\Gamma,x:\sigma,\Gamma'\vdash M:\tau}
\]

\[
\frac{\Gamma,\Gamma'\vdash M\Rrightarrow M':\sigma}{\Gamma,x:\sigma,\Gamma'\vdash M\Rrightarrow M':\sigma}
\]

\[
\frac{\Gamma,\Gamma'\vdash M\Rrightarrow_{\ast}M':\sigma}{\Gamma,x:\sigma,\Gamma'\vdash M\Rrightarrow_{\ast}M':\sigma}
\]

\[
\frac{\Gamma,\Gamma'\vdash M\equiv M':\tau}{\Gamma,x:\sigma,\Gamma'\vdash M\equiv M':\tau}
\]

\[
\frac{\Gamma,\Gamma'\vdash\Delta:\overline{*}}{\Gamma,x:\sigma,\Gamma'\vdash\Delta:\overline{*}}
\]

\[
\frac{\Gamma,\Gamma'\vdash\overline{M}:\Delta}{\Gamma,x:\sigma,\Gamma'\vdash\overline{M}:\Delta}
\]

\[
\frac{\Gamma,\Gamma'\vdash\overline{M}\Rrightarrow\overline{M'}:\Delta}{\Gamma,x:\sigma,\Gamma'\vdash\overline{M}\Rrightarrow\overline{M'}:\Delta}
\]

by mutual induction on the derivations.

\subsubsection{$\Rrightarrow$ is reflexive}

The following rule is admissible:

\[
\frac{\Gamma\vdash M:\sigma}{\Gamma\vdash M\Rrightarrow\,M:\sigma}\,\textrm{\ensuremath{\Rrightarrow}-refl}
\]

\[
\frac{\Gamma\vdash\overline{M}:\Delta}{\Gamma\vdash\overline{M}\Rrightarrow\,\overline{M}:\Delta}\,\textrm{\ensuremath{\Rrightarrow}-refl'}
\]

by induction

\subsubsection{$\equiv$ is reflexive}

The following rule is admissible:

\[
\frac{\Gamma\vdash M:\sigma}{\Gamma\vdash M\equiv M:\sigma}\,\textrm{\ensuremath{\equiv}-refl}
\]

by $\,\textrm{\ensuremath{\Rrightarrow\ast}-refl}$

\subsubsection{Context substitution}

For any derivation of $\Gamma\vdash N:\tau$ the following rules are
admissible:

\[
\frac{\Gamma,x:\tau,\Gamma'\vdash}{\Gamma,\Gamma'\left[x\coloneqq N\right]\vdash}
\]

\[
\frac{\Gamma,x:\tau,\Gamma'\vdash M:\sigma}{\Gamma,\Gamma'\left[x\coloneqq N\right]\vdash M\left[x\coloneqq N\right]\,:\,\sigma\left[x\coloneqq N\right]}
\]

\[
\frac{\Gamma,x:\tau,\Gamma'\vdash M\Rrightarrow M':\sigma}{\Gamma,\Gamma'\left[x\coloneqq N\right]\vdash M\left[x\coloneqq N\right]\Rrightarrow M'\left[x\coloneqq N\right]:\sigma\left[x\coloneqq N\right]}
\]

\[
\frac{\Gamma,x:\tau,\Gamma'\vdash M\Rrightarrow_{\ast}M':\sigma}{\Gamma,\Gamma'\left[x\coloneqq N\right]\vdash M\left[x\coloneqq N\right]\Rrightarrow_{\ast}M'\left[x\coloneqq N\right]:\sigma}
\]

\[
\frac{\Gamma,x:\tau,\Gamma'\vdash M\equiv M':\sigma}{\Gamma,\Gamma'\left[x\coloneqq N\right]\vdash M\left[x\coloneqq N\right]\,\equiv\,M'\left[x\coloneqq N\right]:\sigma\left[x\coloneqq N\right]}
\]

\[
\frac{\Gamma,x:\tau,\Gamma'\vdash\Delta:\overline{*}}{\Gamma,\Gamma'\left[x\coloneqq N\right]\vdash\Delta\left[x\coloneqq N\right]\,:\overline{*}}
\]

\[
\frac{\Gamma,x:\tau,\Gamma'\vdash\overline{M}:\Delta}{\Gamma,\Gamma'\left[x\coloneqq N\right]\vdash\overline{M}\left[x\coloneqq N\right]\,:\Delta\left[x\coloneqq N\right]}
\]

\[
\frac{\Gamma,x:\tau,\overline{M}\Rrightarrow\overline{M'}:\Delta}{\Gamma,\Gamma'\left[x\coloneqq N\right]\vdash\overline{M}\left[x\coloneqq N\right]\Rrightarrow\overline{M'}\left[x\coloneqq N\right]:\Delta\left[x\coloneqq N\right]}
\]

by mutual induction on the derivations. Specifically, at every usage
of $x$ from the var rule in the original derivation, replace the
usage of the var rule with the derivation of $\Gamma\vdash N:\tau$
weakened to the context of $\Gamma,\Gamma'\left[x\coloneqq N\right]\vdash N:\tau$,
and apply appropriate reflexivity when needed.

\subsection{Computation}

\subsubsection{$\Rrightarrow$ preserves type of source}

The following rules are admissible:

\[
\frac{\Gamma\vdash N\Rrightarrow N':\tau}{\Gamma\vdash N:\tau}
\]

\[
\frac{\Gamma\vdash\overline{N}\Rrightarrow\overline{N'}:\Delta}{\Gamma\vdash\overline{N}:\Delta}
\]

by mutual induction

\subsubsection{$\Rrightarrow$ substitution }

The following rule is admissible:

\[
\frac{\Gamma,\Delta,\Gamma'\vdash\overline{M}\Rrightarrow\overline{M'}:\varTheta\quad\Gamma\vdash\overline{N}\Rrightarrow\overline{N'}:\Delta}{\Gamma,\Gamma'\left[\Delta\coloneqq\overline{N}\right]\vdash\overline{M}\left[\Delta\coloneqq\overline{N}\right]\Rrightarrow\overline{M'}\left[\Delta\coloneqq\overline{N'}\right]:\varTheta\left[\Delta\coloneqq\overline{N}\right]}
\]

by induction on the $\Rrightarrow$ derivations with the corollary

Corollary, the following rule is admissible:

\[
\frac{\Gamma,x:\sigma,\Gamma'\vdash M\Rrightarrow M':\tau\quad\Gamma\vdash N\Rrightarrow N':\sigma}{\Gamma,\Gamma'\left[x\coloneqq N\right]\vdash M\left[x\coloneqq N\right]\Rrightarrow M'\left[x\coloneqq N'\right]:\tau\left[x\coloneqq N\right]}
\]


\subsubsection{$\Rrightarrow$ is confluent}

if $\Gamma\vdash M\Rrightarrow N:\sigma$ and $\Gamma\vdash M\Rrightarrow N':\sigma$
then there exists $P$ such that $\Gamma\vdash N\Rrightarrow P:\sigma$
and $\Gamma\vdash N'\Rrightarrow P:\sigma$

and $\Gamma\vdash\overline{M}\Rrightarrow\,\overline{N}:\Delta$ and
$\Gamma\vdash\overline{M}\Rrightarrow\,\overline{N'}:\Delta$ then
there exists $\overline{P}$ such that $\Gamma\vdash\overline{N}\Rrightarrow\overline{P}:\Delta$
and $\Gamma\vdash\overline{N'}\Rrightarrow\overline{P}:\Delta$

by mutual induction on all possible pairs of reductions ( abusing
notation by suppressing $\Gamma,\sigma,\Delta$ that are constant
throughout)
\begin{itemize}
\item $\Pi\textrm{-E-\ensuremath{\Rrightarrow}}$ and $\Pi\textrm{-\ensuremath{\Rrightarrow}}$
\begin{itemize}
\item $M$ is $\left(\mathsf{fun}\,f:\left(x.\tau\right).\,x:\sigma.B\right)\,A$ 
\item $N$ is $\left(\mathsf{fun}\,f:\left(x.\tau\right).\,x:\sigma.B'\right)\,A'$
, $B\Rrightarrow B'$ , $A\Rrightarrow A'$
\item $N'$ is $B''\left[x\coloneqq A'',f\coloneqq\left(\mathsf{fun}\,f:\left(x.\tau\right).\,x:\sigma.B''\right)\right]$
, $B\Rrightarrow B''$ , $A\Rrightarrow A''$
\item $B\Rrightarrow B_{v}$, $A\Rrightarrow A_{v}$ by I.H 
\item $\left(\mathsf{fun}\,f:\left(x.\tau\right).\,x:\sigma.B\right)\,A\Rrightarrow B_{v}\left[x\coloneqq A_{v},f\coloneqq\left(\mathsf{fun}\,f:\left(x.\tau\right).\,x:\sigma.B_{v}\right)\right]$
by repeated $\Rrightarrow$ substitution 
\end{itemize}
\item $D\textrm{-E\textrm{-\ensuremath{\Rrightarrow}}}$ and $D\textrm{-\ensuremath{\Rrightarrow}}$
\begin{itemize}
\item $M$ is $\mathsf{Case}_{x:D\,\overline{y}.\sigma}\,\left(d\,\overline{A}\right)\,\mathsf{of}\left\{ \overline{d_{i}\overline{x}_{i}\Rightarrow B_{i}\,|}\right\} $
\item $N$ is $\mathsf{Case}_{x:D\,\overline{y}.\sigma}\,\left(d\,\overline{A'}\right)\,\mathsf{of}\left\{ \overline{d_{i}\overline{x}_{i}\Rightarrow B'_{i}\,|}\right\} $,
$\overline{A}\Rrightarrow\overline{A'}$, $\forall i.\,B{}_{i}\Rrightarrow B'_{i}$
\item $N'$ is $B''\left[\overline{x}\coloneqq\overline{A''}\right]$, $\overline{A}\Rrightarrow\overline{A''}$,
$B\Rrightarrow B''$, $d\overline{x}\Rightarrow B\in_{i}\left\{ \overline{d_{i}\overline{x}_{i}\Rightarrow B_{i}\,|}\right\} $
\item $B\Rrightarrow B_{v}$, $\overline{A}\Rrightarrow\overline{A_{v}}$
by I.H 
\item $\mathsf{Case}_{x:D\,\overline{y}.\sigma}\,\left(d\,\overline{A}\right)\,\mathsf{of}\left\{ \overline{d_{i}\overline{x}_{i}\Rightarrow B_{i}\,|}\right\} \Rrightarrow B_{v}\left[\overline{x}\coloneqq\overline{A_{v}}\right]$
by repeated $\Rrightarrow$ substitution
\end{itemize}
\item all other reductions match, and follow immediately from induction,
or are symmetric to already presented cases
\end{itemize}

\subsection{$\Rrightarrow_{\ast}$}

\subsubsection{$\Rrightarrow_{\ast}$ is transitive}

The following rule is admissible:

\[
\frac{\Gamma\vdash M\Rrightarrow_{\ast}\,M':\sigma\quad\Gamma\vdash M'\Rrightarrow_{\ast}M'':\sigma}{\Gamma\vdash M\Rrightarrow_{\ast}\,M':\sigma}\,\textrm{\ensuremath{\Rrightarrow\ast}-trans}
\]

by induction

\subsubsection{$\Rrightarrow$ preserves type in source}

The following rules are admissible:

\[
\frac{\Gamma\vdash N\Rrightarrow N':\tau}{\Gamma\vdash N':\tau}
\]

\[
\frac{\Gamma\vdash\overline{N}\Rrightarrow\overline{N'}:\Delta}{\Gamma\vdash\overline{N'}:\Delta}
\]

By induction on the $\Rrightarrow$ derivation with the help of the
substitution lemma.
\begin{itemize}
\item $\Pi\textrm{-\ensuremath{\Rrightarrow}}$
\begin{itemize}
\item $M'\left[x\coloneqq N',f\coloneqq\left(\mathsf{fun}\,f:\left(x.\tau\right).\,x:\sigma.M'\right)\right]\,:\,\tau\left[x\coloneqq N\right]$
by the substitution lemma used on the inductive hypotheses
\end{itemize}
\item $D\textrm{-\ensuremath{\Rrightarrow}}$
\begin{itemize}
\item $O'\left[\overline{x}\coloneqq\overline{N'}\right]:\sigma\left[x\coloneqq d\overline{x}_{i},\overline{y}\coloneqq\overline{N}\right]$
by the substitution lemma used on the inductive hypotheses
\end{itemize}
\item all other cases are trivial
\end{itemize}

\subsubsection{$\Rrightarrow_{\ast}$ preserves type}

The following rule is admissible:

\[
\frac{\Gamma\vdash M\Rrightarrow_{\ast}\,M':\sigma}{\Gamma\vdash M:\sigma}
\]

by induction

\[
\frac{\Gamma\vdash M\Rrightarrow_{\ast}\,M':\sigma}{\Gamma\vdash M':\sigma}
\]

by induction

\subsubsection{$\Rrightarrow_{\ast}$ is confluent}

if $\Gamma\vdash M\Rrightarrow_{\ast}\,N:\sigma$ and $\Gamma\vdash M\Rrightarrow_{\ast}\,N':\sigma$
then there exists $P$ such that 

$\Gamma\vdash N\Rrightarrow_{\ast}\,P:\sigma$ and $\Gamma\vdash N'\Rrightarrow_{\ast}\,P:\sigma$

Follows from $\textrm{\ensuremath{\Rrightarrow\ast}-trans}$ and the
confluence of $\Rrightarrow$ using standard techniques

\subsubsection{$\equiv$ is symmetric}

The following rule is admissible:

\[
\frac{\Gamma\vdash M\equiv N:\sigma}{\Gamma\vdash N\equiv M:\sigma}\,\textrm{\ensuremath{\equiv}-sym}
\]

trivial

\subsubsection{$\equiv$ is transitive}

\[
\frac{\Gamma\vdash M\equiv N:\sigma\qquad\Gamma\vdash N\equiv P:\sigma}{\Gamma\vdash M\equiv P:\sigma}\,\textrm{\ensuremath{\equiv}-trans}
\]

by the confluence of $\Rrightarrow_{\ast}$

\subsubsection{$\equiv$ preserves type}

The following rules are admissible:

\[
\frac{\Gamma\vdash M\equiv\,M':\sigma}{\Gamma\vdash M:\sigma}
\]

\[
\frac{\Gamma\vdash M\equiv\,M':\sigma}{\Gamma\vdash M':\sigma}
\]

by the def of $\Rrightarrow_{\ast}$

\subsubsection{Regularity}

The following rule is admissible:

\[
\frac{\Gamma\vdash M:\sigma}{\Gamma\vdash\sigma:\star}
\]

by induction with $\equiv$-preservation for the Conv case

\subsubsection{$\rightsquigarrow$ implies \textmd{$\Rrightarrow$} }

The following rules are admissible:

\[
\frac{\Gamma\vdash M:\sigma\quad M\rightsquigarrow M'}{\Gamma\vdash M\Rrightarrow M':\sigma}
\]

\[
\frac{\Gamma\vdash\overline{M}:\Delta\quad\overline{M}\rightsquigarrow\overline{M'}}{\Gamma\vdash\overline{M}\Rrightarrow\overline{M'}':\Delta}
\]

by induction on $\rightsquigarrow$

\subsubsection{$\rightsquigarrow$ preserves type}

For any derivations of $\Gamma\vdash M:\sigma$, $M\rightsquigarrow M'$,

\[
\Gamma\vdash M':\sigma
\]

since $\rightsquigarrow$ implies $\Rrightarrow$ and $\Rrightarrow$
preserves types

\subsection{Type constructors}

\subsubsection{Type constructors are stable}
\begin{itemize}
\item if $\Gamma\vdash\ast\Rrightarrow M:\sigma$ then $M$ is $\ast$
\item if $\Gamma\vdash\ast\Rrightarrow_{\ast}M:\sigma$ then $M$ is $\ast$
\item if $\Gamma\vdash\Pi x:\sigma.\tau\Rrightarrow M:\sigma$ then $M$
is $\Pi x:\sigma'.\tau'$ for some $\sigma',\tau'$
\item if $\Gamma\vdash\Pi x:\sigma.\tau\Rrightarrow_{\ast}M:\sigma$ then
$M$ is $\Pi x:\sigma'.\tau'$ for some $\sigma',\tau'$
\item if $\Gamma\vdash D\,\overline{M}\Rrightarrow M:\sigma$ then $M$
is $D\,\overline{M'}$ for some $\overline{M'}$
\item if $\Gamma\vdash D\,\overline{M}\Rrightarrow_{\ast}M:\sigma$ then
$M$ is $D\,\overline{M'}$ for some $\overline{M'}$
\end{itemize}
by induction on the respective relations

\subsubsection{Type constructors definitionaly unique}

There is no derivation of 
\begin{itemize}
\item $\Gamma\vdash\ast\equiv\Pi x:\sigma.\tau\,:\sigma'$ for any $\Gamma,\sigma,\tau,\sigma'$
\item $\Gamma\vdash\ast\equiv D\,\overline{M}\,:\sigma'$ for any $\Gamma,\overline{M},\sigma'$
\item $\Gamma\vdash\Pi x:\sigma.\tau\equiv D\,\overline{M}:\sigma'$ for
any $\Gamma,\sigma,\tau,\overline{M},\sigma'$
\item $\Gamma\vdash D\,\overline{M}\equiv D'\,\overline{N}:\sigma'$ , $D\neq D'$
for any $\Gamma,\overline{M},\overline{N},\sigma'$
\end{itemize}
from $\equiv\textrm{-Def}$ and constructor stability

\subsection{Canonical forms}

If $\Xi\vdash v:\sigma$ then 
\begin{itemize}
\item if $\sigma$ is $\star$ then $v$ is $\star$ , $\Pi x:\sigma.\tau$
or $D\,\overline{M}$ 
\item if $\sigma$ is $\Pi x:\sigma'.\tau$ for some $\sigma'$, $\tau$
then $v$ is $\mathsf{fun}\,f:\left(x.\tau'\right).\,x:\sigma''.P'$
for some $\tau'$, $\sigma''$, $P'$
\item if $\sigma$ is $D\,\overline{M}$ for some $\overline{M}$ then $v$
is $d_{k}\,\overline{v}$ for some $\mathsf{data}\,D\,\Delta\,\mathsf{where}\,\left\{ \overline{d_{i}\,\varTheta_{i}\rightarrow D\overline{M}_{i}\,|}\right\} \in\Xi$
and $d_{k}\,\varTheta_{k}\rightarrow D\overline{M}_{k}\in\overline{d_{i}\,\varTheta_{i}\rightarrow D\overline{M}_{i}\,|}$
\end{itemize}
By induction on the typing derivation
\begin{itemize}
\item Conv,
\begin{itemize}
\item if $\sigma$ is $\star$ then eventually, it was typed with type-in-type,
$\Pi\textrm{-F}$, $D\textrm{-F}$,or $D\textrm{-F}'$. It could not
have been typed by $\Pi\textrm{-I}$ or $D\textrm{-I}$ since constructors
are definitionaly unique
\item if $\sigma$ is $\Pi x:\sigma'.\tau$ then eventually, it was typed
with $\Pi\textrm{-I}$. it could not have been typed b type-in-type,
$\Pi\textrm{-F}$, $D\textrm{-F}$, $D\textrm{-F'}$, or $D\textrm{-I}$
since constructors are definitionaly unique
\item if $\sigma$ is $D\,\overline{M}$ then eventually, it was typed with
$D\textrm{-I}$. it could not have been typed b type-in-type, $\Pi\textrm{-F}$,
$D\textrm{-F}$, $D\textrm{-F'}$, or $\Pi\textrm{-I}$ since constructors
are definitionaly unique
\item can never eventually type with $\Pi\textrm{-E}$, or $D\textrm{-E}$,
since those cannot type values in the empty ctx
\end{itemize}
\item type-in-type, $\Xi\vdash v:\sigma$  is $\Xi\vdash\star:\star$ 
\item $\Pi\textrm{-F}$, $\Xi\vdash v:\sigma$  is $\Xi\vdash\Pi x:\sigma.\tau\,:\star$ 
\item $D\textrm{-F}$, $\Xi\vdash v:\sigma$ is $\Xi\vdash D\,\overline{M}:\star$ 
\item $D\textrm{-F}'$, $\Xi\vdash v:\sigma$ is $\Xi\vdash D\,\overline{M}:\star$ 
\item $\Pi\textrm{-I}$, $\Xi\vdash v:\sigma$  is $\Xi\vdash\mathsf{fun}\,f:\left(x.\tau\right).\,x:\sigma.M\,:\,\varPi x:\sigma.\tau$ 
\item $D\textrm{-I}$, $\Xi\vdash v:\sigma$  is $d\,\overline{N}\,:\,D\,\overline{M}'$
for some $\overline{M}'$
\item no other typing rules are applicable
\end{itemize}

\subsection{Progress}

$\Xi\vdash M:\sigma$ implies that $M$ is a value or there exists
$N$ such that $M\rightsquigarrow N$ and $\Xi\vdash\overline{M}:\Delta$
implies that $\overline{M}$ is a list of values or there exists $\overline{N}$
such that $\overline{M}\rightsquigarrow\overline{N}$

By mutual induction on the typing derivation and list typing derivation

Explicitly:
\begin{itemize}
\item $M$ is typed by the conversion rule, then by \textbf{induction},
$M$ is a value or there exists $N$ such that $M\rightsquigarrow N$ 
\item $M$ cannot be typed by the variable rule in the empty context
\item $M$ is typed by type-in-type. $M$ is $\star$, a value
\item $M$ is typed by $\Pi\textrm{-F}$. $M$ is $\Pi x:\sigma.\tau$,
a value
\item $M$ is typed by $\Pi\textrm{-I}$. $M$ is $\mathsf{fun}\,f:\left(x.\tau\right).\,x:\sigma.M'$,
a value
\item $M$ is typed by $\Pi\textrm{-E}$. $M$ is $P\,N$ then there exist
some $\sigma,\tau$ for $\Xi\vdash P:\Pi x:\sigma.\tau$ and $\Xi\vdash N:\sigma$.
By \textbf{induction} (on the $P$ branch of the derivation) $P$
is a value or there exists $P'$ such that $P\rightsquigarrow P'$.
By \textbf{induction} (on the $N$ branch of the derivation) $N$
is a value or there exists $N'$ such that $N\rightsquigarrow N'$
\begin{itemize}
\item if $P$ is a value then by \textbf{canonical forms}, $P$ is$\mathsf{fun}\,f:\left(x.\tau\right).\,x:\sigma.P'$
and 
\begin{itemize}
\item if $N$ is a value then the one step reduction is $\left(\mathsf{fun}\,f:\left(x.\tau\right).\,x:\sigma.P'\right)\,N\,\rightsquigarrow\,P'\left[x\coloneqq N,f\coloneqq\mathsf{fun}\,f:\left(x.\tau\right).\,x:\sigma.M\right]$ 
\item otherwise there exists $N'$ such that $N\rightsquigarrow N'$, and
the one step reduction is $\left(\mathsf{fun}\,f:\left(x.\tau\right).\,x:\sigma.P'\right)\,N\,\rightsquigarrow\,\left(\mathsf{fun}\,f:\left(x.\tau\right).\,x:\sigma.P'\right)\,N'$ 
\end{itemize}
\item otherwise, there exists $P'$ such that $P\rightsquigarrow P'$ and
the one step reduction is $P\,N\rightsquigarrow P'\,N$
\end{itemize}
\item $M$ is typed by $D\textrm{-F'}$. $M$ is $D\,\overline{N}$, a value
\item $M$ is typed by $D\textrm{-F}$. $M$ is $D\,\overline{N}$, a value
\item $M$ is typed by $D\textrm{-I}$. By \textbf{induction} on lists
\item $M$ is typed by $D\textrm{-E}$. $M$ is $\mathsf{Case}_{x:D\,\overline{y}.\sigma}\,N\,\mathsf{of}\left\{ \overline{d_{i}\overline{x}_{i}\Rightarrow O_{i}\,|}\right\} $
By \textbf{induction} (on the $N$ branch of the derivation) $N$
is a value or there exists $N'$ such that $N\rightsquigarrow N'$
\begin{itemize}
\item if $N$ is a value, by \textbf{canonical forms} $N$ is $d_{k}\,\overline{v}$.
from the typing derivation we know that there is a $d_{k}$ clause
in the case expression. The 1 step reduction is $\mathsf{Case}_{x:D\,\overline{y}.\sigma}\,\left(d_{k}\,\overline{v}\right)\,\mathsf{of}\left\{ \overline{d_{i}\overline{x}_{i}\Rightarrow O_{i}\,|}\right\} \rightsquigarrow O_{k}\left[\overline{x}\coloneqq\overline{v}\right]$
\item otherwise, the one step reduction is $\mathsf{Case}_{x:D\,\overline{y}.\sigma}\,N\,\mathsf{of}\left\{ \overline{d_{i}\overline{x}_{i}\Rightarrow O_{i}\,|}\right\} \rightsquigarrow\mathsf{Case}_{x:D\,\overline{y}.\sigma}\,N'\,\mathsf{of}\left\{ \overline{d_{i}\overline{x}_{i}\Rightarrow O_{i}\,|}\right\} $
\end{itemize}
\item $\overline{M}$ is typed by $\Delta\textrm{-Trm-Emp}$. $\overline{M}$
is $\lozenge$ a degenerate value
\item $\overline{M}$ is typed by $\Delta\textrm{-Trm-+}$. 
\begin{itemize}
\item $\overline{M}$ is a list of values
\item $\overline{M}$ is $\overline{v},N,\overline{N'}$. By \textbf{induction}
\end{itemize}
\end{itemize}

\subsection{Type Soundness}

For any well typed term in an empty context, no sequence of small
step reductions will cause result in a computation to ``get stuck''.
Either a final value will be reached or further reductions can be
taken. This follows by iterating the progress and preservation lemmas.

\section{Conjectured properties}

telescope regularity

\[
\frac{\Gamma\vdash\overline{M}:\varDelta}{\Gamma\vdash\varDelta:\overline{\star}}
\]


\section{Non-Properties}
\begin{itemize}
\item decidable type checking
\item normalization/logical soundness
\end{itemize}

\section{Differences from implementation}

differences from Agda development
\begin{itemize}
\item In Agda presentation only handles functions, without data syntax
\item In Agda the parallel reduction relation does not track the original
typing judgment, though this should be equivalent
\item Only proved the function part of the canonical forms lemma
\item As here, standard properties are 
\end{itemize}
differences from prototype
\begin{itemize}
\item bidirectional, type annotations are not always needed on functions
or data
\item top-level definitions of functions and data
\begin{itemize}
\item top-level recursion function recursion is supported
\item top-level data references are supported
\item mutual recursion is allowed much more than in this presentation
\end{itemize}
\item data constructors use re-use function application parameters rather
then having a list of sub-terms 
\item aside from establishing that a term has a type, type annotations are
not relevant for definitional equality in the prototype
\end{itemize}

\section{Proof improvements}
\begin{itemize}
\item abstract types subtly break the canonical forms lemma
\item Clarify what unsoundness means 
\item proof outline at the top of document
\item better function notation
\item meta syntax to quantify over contextual judgments
\item meta syntax to quantify over $\Rrightarrow$ judgments
\item clean up syntax
\begin{itemize}
\item move to the more modern (a:M)-> N, instead of pi
\item clean up the case matching a bit
\end{itemize}
\item make at terms represented by Latin characters, reserving the geek
letters for other constructs
\item enumerate the syntactic abbreviations
\item Single (or double args) instead of the messy arg list notation 
\end{itemize}

\end{document}
